box and unbox stubs

crypto_hst/Hacl.Constants.fst
@@ -1,89 +1,98 @@
 module Hacl.Constants
 
-open Platform.Bytes
+(* Type abbreviations *)
+type u8  = FStar.UInt8.t
+type u32 = FStar.UInt32.t
+type u64 = FStar.UInt64.t
 
+type uint8_p = FStar.Buffer.buffer u8
 
+(* Size constants (for specifications) *)
+let crypto_box_NONCEBYTES     = 4
+let crypto_box_PUBLICKEYBYTES = 32
+let crypto_box_SECRETKEYBYTES = 32
+let crypto_box_MACBYTES       = 32
 
-(* Type for plaintext data and ciphertext *)
-new type plaintext
-new type ciphertext
+let crypto_secretbox_NONCEBYTES = 4
+let crypto_secretbox_KEYBYTES   = 32
+let crypto_secretbox_MACBYTES   = 32
 
-(* Define hash algorithms *)
-type hash_alg = 
-  | SHA1 
-  | SHA224 
-  | SHA256 
-  | SHA384 
-  | SHA512
+(* (\* Define hash algorithms *\) *)
+(* type hash_alg =  *)
+(*   | SHA1  *)
+(*   | SHA224  *)
+(*   | SHA256  *)
+(*   | SHA384  *)
+(*   | SHA512 *)
 
-(* Define block cipher algorithms *)
-type block_cipher = 
-  | AES_128_CTR 
-  | AES_256_CTR
+(* (\* Define block cipher algorithms *\) *)
+(* type block_cipher =  *)
+(*   | AES_128_CTR  *)
+(*   | AES_256_CTR *)
 
-(* Define AEAD cipher algorithms *)
-type aead_cipher = 
-  | AES_128_GCM 
-  | AES_256_GCM
-  | XSALSA20_POLY1305
-  | SALSA20_POLY1305
-  | CHACHA20_POLY1305
+(* (\* Define AEAD cipher algorithms *\) *)
+(* type aead_cipher =  *)
+(*   | AES_128_GCM  *)
+(*   | AES_256_GCM *)
+(*   | XSALSA20_POLY1305 *)
+(*   | SALSA20_POLY1305 *)
+(*   | CHACHA20_POLY1305 *)
 
-(* Define elliptic curves algorithms *)
-type ec_curve =
-  | ECC_P256
-  | ECC_Curve25519
-  | ECC_Ed448
+(* (\* Define elliptic curves algorithms *\) *)
+(* type ec_curve = *)
+(*   | ECC_P256 *)
+(*   | ECC_Curve25519 *)
+(*   | ECC_Ed448 *)
 
-(* Define elliptic cureve parameters *)
-type ec_params = {
-  curve: ec_curve;
-  point_compression: bool;
-}
+(* (\* Define elliptic cureve parameters *\) *)
+(* type ec_params = { *)
+(*   curve: ec_curve; *)
+(*   point_compression: bool; *)
+(* } *)
 
-(* Define an elliptic curve point *)
-type ec_point = {
-  ecx : bytes;
-  ecy : bytes;
-}
+(* (\* Define an elliptic curve point *\) *)
+(* noeq type ec_point = { *)
+(*   ecx : uint8_p; *)
+(*   ecy : uint8_p; *)
+(* } *)
 
-(* Define a SKE key *)
-type key
+(* (\* Define a SKE key *\) *)
+(* type key *)
 
-(* Define a PKE key *)
-type ec_key = {
-  ec_params : ec_params;
-  ec_point : ec_point;
-  ec_priv : option bytes;
-}
+(* (\* Define a PKE key *\) *)
+(* type ec_key = { *)
+(*   ec_params : ec_params; *)
+(*   ec_point : ec_point; *)
+(*   ec_priv : option uint8_p; *)
+(* } *)
 
-(* Functions returning key,iv and tag sizes for AEAD ciphers *)
-let aeadKeySize = function
-  | AES_128_GCM -> 16
-  | AES_256_GCM -> 32
+(* (\* Functions returning key,iv and tag sizes for AEAD ciphers *\) *)
+(* let aeadKeySize = function *)
+(*   | AES_128_GCM -> 16ul *)
+(*   | AES_256_GCM -> 32ul *)
 
-let aeadRealIVSize = function
-  | AES_128_GCM -> 12
-  | AES_256_GCM -> 12
+(* let aeadRealIVSize = function *)
+(*   | AES_128_GCM -> 12ul *)
+(*   | AES_256_GCM -> 12ul *)
 
-let aeadTagSize = function
-  | AES_128_GCM -> 16
-  | AES_256_GCM -> 16
+(* let aeadTagSize = function *)
+(*   | AES_128_GCM -> 16ul *)
+(*   | AES_256_GCM -> 16ul *)
  
-(* Function returning the length in bytes of a hash result *)
-val hashSize: hash_alg -> Tot nat
-let hashSize = function
-  | SHA1 -> 20
-  | SHA224 -> 28
-  | SHA256 -> 32
-  | SHA384 -> 48
-  | SHA512 -> 64
+(* (\* Function returning the length in bytes of a hash result *\) *)
+(* val hashSize: hash_alg -> Tot FStar.UInt32.t *)
+(* let hashSize = function *)
+(*   | SHA1 -> 20ul *)
+(*   | SHA224 -> 28ul *)
+(*   | SHA256 -> 32ul *)
+(*   | SHA384 -> 48ul *)
+(*   | SHA512 -> 64ul *)
 
 
-(* Serializing and parsing functions for ec_point and ec_key *)
-assume val serialize_ec_point: ec_point -> Tot bytes
-assume val serialize_ec_key: ec_key -> Tot bytes
-assume val parsing_ec_point: bytes -> Tot ec_point
-assume val parsing_ec_key: bytes -> Tot ec_key
-assume val ec_point_is_on_curve: ec_curve -> ec_point -> Tot bool
-assume val ec_point_is_pkey_of_skey: ec_curve -> ec_key -> ec_point -> Tot bool
+(* (\* Serializing and parsing functions for ec_point and ec_key *\) *)
+(* assume val serialize_ec_point: ec_point -> Tot uint8_p *)
+(* assume val serialize_ec_key: ec_key -> Tot uint8_p *)
+(* assume val parsing_ec_point: uint8_p -> Tot ec_point *)
+(* assume val parsing_ec_key: uint8_p -> Tot ec_key *)
+(* assume val ec_point_is_on_curve: ec_curve -> ec_point -> Tot bool *)
+(* assume val ec_point_is_pkey_of_skey: ec_curve -> ec_key -> ec_point -> Tot bool *)
