crypto_hst/Hacl.Box.fst
@@ -1,0 +1,63 @@
+module Hacl.Box
+
+open FStar.Buffer
+open FStar.HST
+open Hacl.Constants
+
+
+(* Module abbreviations *)
+module HS  = FStar.HyperStack
+module B   = FStar.Buffer
+module U8  = FStar.UInt8
+module U32 = FStar.UInt32
+module U64 = FStar.UInt64
+
+
+val crypto_box_easy:
+  c:uint8_p ->
+  m:uint8_p ->
+  mlen:u64{let len = U64.v mlen in length c = len + crypto_box_MACBYTES /\ len = length m}  ->
+  n:uint8_p{length n = crypto_box_NONCEBYTES} ->
+  pk:uint8_p{length pk = crypto_box_PUBLICKEYBYTES} ->
+  sk:uint8_p{length sk = crypto_box_SECRETKEYBYTES} ->
+  Stack u32
+    (requires (fun h -> live h c /\ live h m /\ live h n /\ live h pk /\ live h sk))
+    (ensures  (fun h0 z h1 -> modifies_1 c h0 h1 /\ live h1 c))
+
+
+val crypto_box_open_easy:
+  m:uint8_p ->
+  c:uint8_p ->
+  mlen:u64{let len = U64.v mlen in length m = len - crypto_box_MACBYTES /\ len = length c}  ->
+  n:uint8_p{length n = crypto_box_NONCEBYTES} ->
+  pk:uint8_p{length pk = crypto_box_PUBLICKEYBYTES} ->
+  sk:uint8_p{length sk = crypto_box_SECRETKEYBYTES} ->
+  Stack u32
+    (requires (fun h -> live h c /\ live h m /\ live h n /\ live h pk /\ live h sk))
+    (ensures  (fun h0 z h1 -> modifies_1 c h0 h1 /\ live h1 c))
+
+
+val crypto_box_detached:
+  c:uint8_p ->
+  mac:uint8_p{length mac = crypto_box_MACBYTES} ->
+  m:uint8_p ->
+  mlen:u64{let len = U64.v mlen in length c = len /\ len = length m}  ->
+  n:uint8_p{length n = crypto_box_NONCEBYTES} ->
+  pk:uint8_p{length pk = crypto_box_PUBLICKEYBYTES} ->
+  sk:uint8_p{length sk = crypto_box_SECRETKEYBYTES} ->
+  Stack u32
+    (requires (fun h -> live h c /\ live h m /\ live h n /\ live h pk /\ live h sk))
+    (ensures  (fun h0 z h1 -> modifies_1 c h0 h1 /\ live h1 c))
+
+
+val crypto_box_open_easy:
+  m:uint8_p ->
+  c:uint8_p ->
+  mac:uint8_p{length mac = crypto_box_MACBYTES} ->
+  mlen:u64{let len = U64.v mlen in length m = len /\ len = length c}  ->
+  n:uint8_p{length n = crypto_box_NONCEBYTES} ->
+  pk:uint8_p{length pk = crypto_box_PUBLICKEYBYTES} ->
+  sk:uint8_p{length sk = crypto_box_SECRETKEYBYTES} ->
+  Stack u32
+    (requires (fun h -> live h c /\ live h m /\ live h n /\ live h pk /\ live h sk))
+    (ensures  (fun h0 z h1 -> modifies_1 c h0 h1 /\ live h1 c))
